Prove correspondence of abstract and storage states
Also:
- Add procedure heap to the storage state [not fully proved yet]
- Start to formalize Register procedure system call
- Add syntax highlighting to the pdf version
- Refactoring

Cap9.thy
@@ -11,11 +11,20 @@ subsection \<open>Procedure keys\<close>
 
 text \<open>
   Procedure keys are represented as 24-byte (192 bits) machine words.
-  Keys will be used both in the abstract and concrete state.
+  Keys will be used both in the abstract and concrete states.
 \<close>
 
 type_synonym word24 = "192 word"
 type_synonym key = word24
+
+text \<open>
+  Instantiate @{class len0} type class to extract lengths from the @{type key} and other word
+  types avoiding repeated explicit numeric specification of the length.
+\<close>
+instantiation word :: (len0) len0 begin
+definition len_word[simp]: "len_of (_ :: 'a::len0 word itself) = LENGTH('a)"
+instance ..
+end
 
 text \<open>
   We make some assumptions about the set of all procedures that can be registered in the system:
@@ -24,68 +33,73 @@ text \<open>
   \item this function is injective on the set;
   \item number of all procedures is smaller or equal to the number of all keys.
   \end{enumerate}
-  We accomplish it by using Isar type classes:
+  The assumptions concretize our hypothesis about the absence of procedure key collisions.
+  We formalize these assumptions by defining a corresponding Isar type class of allowed
+  procedures:
 \<close>
 
 class proc_class =
   fixes key :: "'a \<Rightarrow> key"
   assumes "CARD ('a) \<le> CARD (key)"
-  assumes "inj key"
+  assumes key_inj:"inj key"
 
 text \<open>
   To insure we don't introduce contradictions with these assumptions we build a sample model
-  of the set of all procedures. To do this we proceed with some additional definitions.
+  of the set of all procedures. Although here use a relatively simple hash function, we
+  don't impose any additional requirements on the function, so it can be replaced with any real
+  cryptographic hash. We only need a single procedure-key pair to be calculated in advance, which
+  is easily achievable by computing the hash of some trivial allowed procedure.
+
+  We proceed with the corresponding definitions.
 \<close>
+
+subsection \<open>Dummy hash function\<close>
 
 text \<open>Byte is 8-bit machine word:\<close>
 type_synonym byte = "8 word"
 
-subsection \<open>Hash function\<close>
-
 text \<open>
-  This is a hash function that takes an arbitrary list of bytes and returns its 24-byte hash.
-  It is used to obtain procedure keys.
+  As an example we use a simple @{text djb2} hash function to compute 24-byte hash
+  of a list of bytes.
 \<close>
 
-fun hash_rec :: "nat \<Rightarrow> byte list \<Rightarrow> key" where
-  "hash_rec n []             = 0" |
-  "hash_rec 0 [e]            = ucast e << 191" |
-  "hash_rec (Suc n) [e]      = ucast e << n" |
-  "hash_rec 0 (e # es)       = (ucast e << 191) XOR hash_rec 191 es" |
-  "hash_rec (Suc n) (e # es) = (ucast e << n) XOR hash_rec n es"
-
-definition "some_hash \<equiv> hash_rec 0"
+abbreviation "seed :: key \<equiv> 5381"
+fun djb2 :: "byte list \<Rightarrow> key" where
+  "djb2 []    =    seed" |
+  "djb2 (e # es)    =    (let h = djb2 es in (h << 5) + h + ucast e)"
 
 text \<open>
-  This is an auxiliary function that takes some hash as an input and if there is some byte list
-  (called "element"), whose hash matches the input, then the function will return it.
-  Otherwise, the function returns an empty set:
+  To formalize a notion of a set of procedures without hash collisions we nonconstructively
+  define a choice function to select exactly one arbitrary procedure for each possible key. In
+  reality this corresponds to the assumption that we never encounter hash collisions, so the
+  choice function can be assumed to be always well-defined on the current set of
+  procedure keys since the Hilbert epsilon operator's choice is arbitrary.
 \<close>
 
 definition "choose_proc k \<equiv>
-  if k = 0                     then {[]}
-  else if \<exists> p. some_hash p = k then {SOME p. some_hash p = k}
-  else                              {}"
+  if k = seed then
+    {[]}
+  else if \<exists> p. djb2 p = k then
+    {SOME p. djb2 p = k}
+  else
+    {}"
 
-lemma choose_proc[simp]: "x \<in> choose_proc k \<Longrightarrow> some_hash x = k"
+lemma choose_proc[simp]: "x \<in> choose_proc k \<Longrightarrow> djb2 x = k"
   unfolding choose_proc_def
-  by (auto simp add: some_hash_def split: if_splits intro: someI)
+  by (auto split: if_splits intro: someI)
 
-text \<open>Each key has only one corresponding procedure:\<close>
-
+text \<open>The procedure corresponding to each key is unique.\<close>
 lemma[simp]: "\<lbrakk>x \<in> choose_proc k; y \<in> choose_proc k\<rbrakk> \<Longrightarrow> x = y"
   unfolding choose_proc_def
   by (simp split: if_splits)
 
-subsection \<open>Procedures\<close>
+subsection \<open>Dummy set of procedures\<close>
 
-text \<open>@{text Procs} is a set of all possible procedures, hash of which will be a
-      valid procedure key:\<close>
+text \<open>@{text Procs} is a set of all allowed procedures, without procedure key collisions:\<close>
 definition "Procs \<equiv> \<Union>k. choose_proc k"
 
 text \<open>
-  Here we introduce a new type called @{text proc} which will be used to represent procedures in the
-  abstract state. Type @{text proc} is identified with the @{const Procs} set:
+  A new type @{text proc} is the sought instantiation of the @{class proc_class} type class.
 \<close>
 
 typedef proc = Procs
@@ -94,53 +108,52 @@ typedef proc = Procs
 
 subsubsection \<open>Injectivity of the hash function\<close>
 
-text \<open>Hash function is injective on the domain of all procedures:\<close>
-
-lemma some_hash_inj: "inj_on some_hash Procs"
+text \<open>Hash function is injective on the domain of all procedures.\<close>
+lemma djb2_inj: "inj_on djb2 Procs"
   unfolding inj_on_def Procs_def
   by auto
 
 subsubsection \<open>Number of all procedures\<close>
 
-text \<open>Here we introduce maximum number of procedure keys:\<close>
+text \<open>Here we introduce maximum number of registered procedure keys:\<close>
 
-abbreviation "max_nkeys \<equiv>  2 ^ 192 :: nat"
+abbreviation "max_nkeys \<equiv>  2 ^ LENGTH(key) :: nat"
 
-text \<open>Number of all procedures must be equal or smaller then the maximum number of procedure keys:\<close>
+text \<open>Number of all procedures must be equal or smaller then the maximum number of procedure keys.\<close>
 
 lemma card_procs: "card Procs \<le> max_nkeys"
   unfolding Procs_def
 proof (subst card_UN_disjoint)
   show  "finite (UNIV :: key set)"
     and "\<forall>i\<in>UNIV. finite (choose_proc i)"
-    unfolding choose_proc_def some_hash_def
+    unfolding choose_proc_def
     by (simp_all split: if_splits)
   show "\<forall>i\<in>UNIV. \<forall>j\<in>UNIV. i \<noteq> j \<longrightarrow> choose_proc i \<inter> choose_proc j = {}"
-    by (auto, ((drule choose_proc)+, simp))
+    by (auto, drule choose_proc, simp)
   show "(\<Sum>i\<in>UNIV. card (choose_proc i)) \<le> max_nkeys"
     using sum_bounded_above[of "UNIV :: key set" "\<lambda> i. card (choose_proc i)", where K = 1]
     unfolding choose_proc_def card_word
     by auto
 qed
 
-subsection \<open>Sample set of procedures\<close>
+subsubsection \<open>Instantiation\<close>
 
 text \<open>
-  Here we show that there is a sample set of all procedures that satisfies all assumptions:
+  Here we show that there the dummy type @{type proc} satisfies our assumptions.
 \<close>
 
 instantiation proc :: proc_class
 begin
-definition "key \<equiv> some_hash \<circ> Rep_proc"
+definition "key \<equiv> djb2 \<circ> Rep_proc"
 
 instance proof
-  show "CARD(proc) \<le> CARD(key)"
+  have "CARD(key) = 2 ^ LENGTH(key)" by (simp add:card_word)
+  thus "CARD(proc) \<le> CARD(key)"
     using card_procs
-          card_word[where 'a = 192]
           type_definition.card[OF proc.type_definition_proc]
     by auto
   show "inj (key :: proc \<Rightarrow> _)"
-    using some_hash_inj proc.Rep_proc proc.Rep_proc_inject
+    using djb2_inj proc.Rep_proc proc.Rep_proc_inject
     unfolding inj_def key_proc_def inj_on_def
     by force
 qed
@@ -165,22 +178,26 @@ text \<open>
 \<close>
 
 text \<open>Number of the procedures in the abstract state:\<close>
-abbreviation "nprocs \<S> \<equiv> card (dom (procs \<S>))"
+abbreviation "nprocs \<sigma> \<equiv> card (dom (procs \<sigma>))"
 
-text \<open>List of procedures keys:\<close>
-abbreviation "proc_keys \<S> \<equiv> dom (procs \<S>)"
+text \<open>List of procedure keys:\<close>
+abbreviation "proc_keys \<sigma> \<equiv> dom (procs \<sigma>)"
+
+text \<open>List of procedure indexes:\<close>
+abbreviation "proc_ids \<sigma> \<equiv> {1..nprocs \<sigma>}"
 
 text \<open>Pair with the procedure index and procedure itself for a given key:\<close>
-abbreviation "proc \<S> k \<equiv> the (procs \<S> k)"
+abbreviation "proc \<sigma> k \<equiv> the (procs \<sigma> k)"
 
 text \<open>Procedure index for a given key:\<close>
-abbreviation "proc_id \<S> k \<equiv> fst (proc \<S> k)"
+abbreviation "proc_id \<sigma> k \<equiv> fst (proc \<sigma> k)"
 
 text \<open>Procedure itself for a given key:\<close>
-abbreviation "proc_bdy \<S> k \<equiv> snd (proc \<S> k)"
+abbreviation "proc_bdy \<sigma> k \<equiv> snd (proc \<sigma> k)"
 
 text \<open>Maximum number of procedures in the abstract state:\<close>
-abbreviation "max_nprocs_nat \<equiv> 2 ^ 24 - 1 :: nat"
+abbreviation "proc_id_len \<equiv> 24"
+abbreviation "max_nprocs \<equiv> 2 ^ proc_id_len - 1 :: nat"
 
 subsubsection \<open>Well-formedness\<close>
 
@@ -194,19 +211,18 @@ text \<open>
   \end{enumerate}
 \<close>
 
-definition "procs_rng_wf \<S> \<equiv>
-  (\<forall> k \<in> proc_keys \<S>. proc_id \<S> k \<in> {1 .. nprocs \<S>} \<and> key (proc_bdy \<S> k) = k) \<and>
-   nprocs \<S> \<le> max_nprocs_nat"
+definition "procs_rng_wf \<sigma> \<equiv>
+  (\<forall> k \<in> proc_keys \<sigma>. proc_id \<sigma> k \<in> proc_ids \<sigma> \<and> key (proc_bdy \<sigma> k) = k) \<and>
+   nprocs \<sigma> \<le> max_nprocs"
 
-text \<open>Procedure indexes must be injective:\<close>
-definition "procs_map_wf \<S> \<equiv> inj_on (proc_id \<S>) (proc_keys \<S>)"
+text \<open>Procedure indexes must be injective.\<close>
+definition "procs_map_wf \<sigma> \<equiv> inj_on (proc_id \<sigma>) (proc_keys \<sigma>)"
 
-text \<open>Abstract state is well-formed if the previous two properties are satisfied:\<close>
-
-definition abs_wf :: "'p :: proc_class abs \<Rightarrow> bool" ("\<turnstile>_" [60]) where
-  "\<turnstile>\<S> \<equiv>
-     procs_rng_wf \<S>
-   \<and> procs_map_wf \<S>"
+text \<open>Abstract state is well-formed if the previous two properties are satisfied.\<close>
+definition abs_wf :: "'p :: proc_class abs \<Rightarrow> bool" ("\<turnstile> _" [60] 60) where
+  "\<turnstile>\<sigma> \<equiv>
+     procs_rng_wf \<sigma>
+   \<and> procs_map_wf \<sigma>"
 
 lemmas procs_rng_wf = abs_wf_def procs_rng_wf_def
 
@@ -214,30 +230,56 @@ lemmas procs_map_wf = abs_wf_def procs_map_wf_def
 
 section \<open>Storage state\<close>
 
-text \<open>32-byte machine words that are used to model keys and values of the storage:\<close>
-
+text \<open>32-byte machine words that are used to model keys and values of the storage.\<close>
 type_synonym word32 = "256 word" (* 32 bytes *)
 
 text \<open>
   Storage is a function that takes a 32-byte word (key) and returns another
-  32-byte word (value):
+  32-byte word (value).
 \<close>
 type_synonym storage = "word32 \<Rightarrow> word32"
 
 text \<open>Storage key that corresponds to the number of procedures in the list:\<close>
-abbreviation "nprocs_key \<equiv> 0xffffffff01 << (27 * 8) :: word32"
+abbreviation nprocs_addr ("@nprocs") where "nprocs_addr \<equiv> 0xffffffff01 << (27 * 8) :: word32"
 
 text \<open>Storage key that corresponds to the procedure key with index i:\<close>
-abbreviation "key_addr_of_id i \<equiv> nprocs_key OR of_nat i"
+definition proc_key_addr ("@proc'_key") where "@proc_key i \<equiv> @nprocs OR of_nat i"
 
 text \<open>Procedure index that corresponds to some procedure key address:\<close>
-abbreviation "id_of_key_addr a \<equiv> unat (nprocs_key XOR a)"
+definition id_of_proc_key_addr where "id_of_proc_key_addr a \<equiv> unat (@nprocs XOR a)"
 
 text \<open>Maximum number of procedures in the kernel, but in the form of a 32-byte machine word:\<close>
-abbreviation "max_nprocs_word \<equiv> 2 ^ 24 - 1 :: word32"
+abbreviation "max_nprocs_word \<equiv> 2 ^ proc_id_len - 1 :: word32"
 
 text \<open>Declare some lemmas as simplification rules:\<close>
 declare unat_word_ariths[simp] word_size[simp]
+
+text \<open>Storage address that corresponds to the procedure heap for a given procedure key:\<close>
+abbreviation "proc_heap_mask \<equiv>  0xffffffff00 << (27 * 8) :: word32"
+abbreviation proc_heap_addr :: "key \<Rightarrow> word32" ("@proc'_heap") where
+  "@proc_heap k \<equiv> proc_heap_mask OR ((ucast k) << (3 * 8))"
+
+text \<open>Storage address that corresponds to the procedure address:\<close>
+abbreviation proc_addr_addr ("@proc'_addr") where "@proc_addr k \<equiv> @proc_heap k"
+
+text \<open>Storage address that corresponds to the procedure index:\<close>
+abbreviation proc_id_addr ("@proc'_id") where "@proc_id k \<equiv> @proc_heap k OR 0x01"
+
+text \<open>Procedure key that corresponds to some procedure index address:\<close>
+abbreviation proc_key_of_id_addr :: "word32 \<Rightarrow> key" where
+  "proc_key_of_id_addr a \<equiv> ucast (proc_heap_mask XOR a)"
+
+text \<open>Storage address that corresponds to the number of capabilities of type @{text t}:\<close>
+abbreviation ncaps_addr :: "key \<Rightarrow> byte \<Rightarrow> word32" ("@ncaps") where
+  "@ncaps k t \<equiv> @proc_heap k OR (ucast t << 2 * 8)"
+
+text \<open>
+  Storage address that corresponds to the capability of type @{text t},
+  with index @{text "i - 1"},
+  and offset @{text off} into that capability:
+\<close>
+abbreviation proc_cap_addr :: "key \<Rightarrow> byte \<Rightarrow> byte \<Rightarrow> byte \<Rightarrow> word32" ("@proc'_cap") where
+  "@proc_cap k t i off \<equiv> @proc_heap k OR (ucast t << 2 * 8) OR (ucast i << 8) OR ucast off"
 
 subsection \<open>Lemmas\<close>
 
@@ -245,22 +287,23 @@ subsubsection \<open>Auxiliary lemmas about procedure key addresses\<close>
 
 text \<open>Valid procedure id has all zeros in its higher bits.\<close>
 lemma proc_id_high_zeros[simp]:
-  "n \<le> max_nprocs_word \<Longrightarrow> \<forall>i\<in>{24..<256}. \<not> n !! i" (is "?nbound \<Longrightarrow> \<forall>_ \<in> ?high. _")
+  "n \<le> max_nprocs_word \<Longrightarrow> \<forall>i\<in>{proc_id_len..<LENGTH(word32)}. \<not> n !! i"
+  (is "?nbound \<Longrightarrow> \<forall>_ \<in> ?high. _")
 proof
   fix i
   assume 0:"i \<in> ?high"
-  from 0 have "2 ^ 24 \<le> (2 :: nat) ^ i" by (simp add: numerals(2))
+  from 0 have "2 ^ proc_id_len \<le> (2 :: nat) ^ i" by (simp add: numerals(2))
   moreover from 0 have "0 < (2 :: word32) ^ i"  by (subst word_2p_lem; simp)
-  ultimately have "2 ^ 24 \<le> (2 :: word32) ^ i"
+  ultimately have "2 ^ proc_id_len \<le> (2 :: word32) ^ i"
     unfolding word_le_def
     by (subst (asm) of_nat_le_iff[symmetric], simp add:uint_2p)
   thus "?nbound \<Longrightarrow> \<not> n !! i"
     unfolding not_def
-    by (intro impI) (frule bang_is_le, unat_arith)
+    by (intro impI) (drule bang_is_le, unat_arith)
 qed
 
 text \<open>Address of the \# of procedures has all zeros in its lower bits.\<close>
-lemma nprocs_key_low_zeros[simp]: "\<forall>i\<in>{0..< 24}. \<not> nprocs_key !! i"
+lemma nprocs_key_low_zeros[simp]: "\<forall>i\<in>{0..<proc_id_len}. \<not> @nprocs !! i"
   by (subst nth_shiftl, auto)
 
 text \<open>
@@ -268,7 +311,9 @@ text \<open>
   a property holds on all bits if and only if it holds on the higher and lower bits.\<close>
 lemma low_high_split:
    "(\<forall>n. P ((x :: word32) !! n)) =
-    ((\<forall>n\<in>{0..<24}. P (x !! n)) \<and> (\<forall>n\<in> {24..<256}. P (x !! n)) \<and> P False)"
+    ((\<forall>n\<in>{0..<proc_id_len}. P (x !! n)) \<and>
+     (\<forall>n\<in>{proc_id_len..<LENGTH(word32)}. P (x !! n)) \<and>
+     P False)"
   (is "?left = ?right")
 proof (intro iffI)
   have "\<not> x !! size x" using test_bit_size[of x "size x"] by blast
@@ -280,7 +325,8 @@ qed
 
 text \<open>Computing procedure key address by its id is an invertible operation.\<close>
 lemma id_of_key_addr_inv[simp]:
-   "i \<le> max_nprocs_nat \<Longrightarrow> id_of_key_addr (key_addr_of_id i) = i" (is "?ibound \<Longrightarrow> ?rev")
+   "i \<le> max_nprocs \<Longrightarrow> id_of_proc_key_addr (@proc_key i) = i"
+   (is "?ibound \<Longrightarrow> ?rev")
 proof-
   assume 0:"?ibound"
   hence 1:"unat (of_nat i :: word32) = i"
@@ -288,64 +334,76 @@ proof-
   hence "of_nat i \<le> max_nprocs_word"
     using 0
     by (simp add: word_le_nat_alt)
-  hence "nprocs_key XOR nprocs_key OR (of_nat i) = of_nat i"
+  hence "@nprocs XOR @nprocs OR (of_nat i) = of_nat i"
     using nprocs_key_low_zeros proc_id_high_zeros
     by (auto simp add: word_eq_iff word_ops_nth_size)
   thus "?rev"
     using 1
+    unfolding proc_key_addr_def id_of_proc_key_addr_def
     by simp
 qed
 
 section \<open>Correspondence between abstract and storage states\<close>
 
-text \<open>Number of procedures is stored by the corresponding address (@{const nprocs_key}).\<close>
-definition "models_nprocs S \<S> \<equiv> unat (S nprocs_key) = nprocs \<S>"
+text \<open>Number of procedures is stored by the corresponding address (@{text "@nprocs"}).\<close>
+definition "models_nprocs s \<sigma> \<equiv> unat (s @nprocs) = nprocs \<sigma>"
 
 text \<open>Each procedure key @{text k} is stored by the corresponding address
-      (@{term "key_addr_of_id k"}).\<close>
-definition "models_proc_keys S \<S> \<equiv>
-  \<forall> k \<in> proc_keys \<S>. S (key_addr_of_id (proc_id \<S> k)) = ucast k"
+      (@{term "@proc_key k"}).\<close>
+definition "models_proc_keys s \<sigma> \<equiv>
+  \<forall> k \<in> proc_keys \<sigma>. s (@proc_key (proc_id \<sigma> k)) = ucast k"
+
+text \<open>For each procedure key @{text k} its index is stored by the corresponding address
+      (@{text "@proc_id k"}).\<close>
+definition "models_proc_ids s \<sigma> \<equiv>
+  \<forall> k \<in> proc_keys \<sigma>. unat (s (@proc_id k)) = proc_id \<sigma> k"
 
 text \<open>A storage corresponds to the abstract state
      if and only if the above properties are satisfied.\<close>
-definition models :: "storage \<Rightarrow> ('p :: proc_class) abs \<Rightarrow> bool" ("_ \<tturnstile> _" [65]) where
-  "S \<tturnstile> \<S> \<equiv>
-    models_nprocs S \<S>
-  \<and> models_proc_keys S \<S>"
+definition models :: "storage \<Rightarrow> ('p :: proc_class) abs \<Rightarrow> bool" ("_ \<tturnstile> _" [65, 65] 65) where
+  "s \<tturnstile> \<sigma> \<equiv>
+    models_nprocs s \<sigma>
+  \<and> models_proc_keys s \<sigma>
+  \<and> models_proc_ids s \<sigma>"
 
 lemmas models_nprocs = models_def models_nprocs_def
-
 lemmas models_proc_keys = models_def models_proc_keys_def
+lemmas models_proc_ids = models_def models_proc_ids_def
 
 text \<open>In the following we aim to proof the existence of a storage corresponding to any
       well-formed abstract state (so that any well-formed abstract state can be encoded
-      and stored). Later we still need to prove that the encoding is unambiguous.
+      and stored). Then prove that the encoding is unambiguous.
 \<close>
 
 subsection \<open>Auxiliary definitions and lemmas\<close>
 
-text \<open>An empty storage.\<close>
-definition "zero_con (_ :: word32) \<equiv> 0 :: word32"
+text \<open>An empty storage:\<close>
+definition "zero_storage (_ :: word32) \<equiv> 0 :: word32"
 
-text \<open>The set of all procedure key addresses.\<close>
-definition "proc_key_addrs \<S> \<equiv> { key_addr_of_id (proc_id \<S> k) | k. k \<in> proc_keys \<S> }"
+text \<open>The set of all procedure key addresses:\<close>
+definition proc_key_addrs ("@proc'_keys") where
+  "@proc_keys \<sigma> \<equiv> { @proc_key (proc_id \<sigma> k) | k. k \<in> proc_keys \<sigma> }"
+
+definition proc_id_addrs ("@proc'_ids") where "@proc_ids \<sigma> \<equiv> { @proc_id k | k. k \<in> proc_keys \<sigma> }"
+(* TODO: add some lemmas? *)
 
 text \<open>Procedure id can be converted to a 32-byte word without overflow.\<close>
 lemma proc_id_inv[simp]:
-  "\<lbrakk>\<turnstile> \<S>; k \<in> proc_keys \<S>\<rbrakk> \<Longrightarrow> unat (of_nat (proc_id \<S> k) :: word32) = proc_id \<S> k"
+  "\<lbrakk>\<turnstile> \<sigma>; k \<in> proc_keys \<sigma>\<rbrakk> \<Longrightarrow> unat (of_nat (proc_id \<sigma> k) :: word32) = proc_id \<sigma> k"
   unfolding procs_rng_wf
   by (force intro:le_unat_uoi[where z=max_nprocs_word])
 
 text \<open>Moreover, any procedure id is non-zero and bounded by the maximum available id
       (@{const max_nprocs_word}).\<close>
 lemma proc_id_bounded[intro]:
-  "\<lbrakk>\<turnstile> \<S>; k \<in> proc_keys \<S>\<rbrakk> \<Longrightarrow>
-    (0 :: word32) < of_nat (proc_id \<S> k) \<and> of_nat (proc_id \<S> k) \<le> max_nprocs_word"
+  "\<lbrakk>\<turnstile> \<sigma>; k \<in> proc_keys \<sigma>\<rbrakk> \<Longrightarrow>
+    (0 :: word32) < of_nat (proc_id \<sigma> k) \<and> of_nat (proc_id \<sigma> k) \<le> max_nprocs_word"
   by (simp add:word_le_nat_alt word_less_nat_alt, force simp add:procs_rng_wf)
 
 text \<open>Since it's non-zero, any procedure id has a non-zero bit in its lower part.\<close>
 lemma proc_id_low_one:
-  "0 < n \<and> n \<le> max_nprocs_word \<Longrightarrow> \<exists>i\<in>{0..<24}. n !! i" (is "?nbound \<Longrightarrow> _")
+  "0 < n \<and> n \<le> max_nprocs_word \<Longrightarrow> \<exists>i\<in>{0..<proc_id_len}. n !! i"
+  (is "?nbound \<Longrightarrow> _")
 proof-
   assume 0:"?nbound"
   hence "\<not> ?thesis \<Longrightarrow> n = 0" by (auto simp add:inc_le intro!:word_eqI)
@@ -354,43 +412,65 @@ proof-
 qed
 
 text \<open>And procedure key address is different from the address of the \# of procedures
-      (@{const nprocs_key}).\<close>
+      (@{text "@nprocs"}).\<close>
 lemma proc_key_addr_neq_nprocs_key:
-  "0 < n \<and> n \<le> max_nprocs_word \<Longrightarrow> nprocs_key OR n \<noteq> nprocs_key" (is "?nbound \<Longrightarrow> _")
+  "0 < n \<and> n \<le> max_nprocs_word \<Longrightarrow> @nprocs OR n \<noteq> @nprocs"
+  (is "?nbound \<Longrightarrow> _")
 proof-
   assume 0:"?nbound"
-  hence "\<exists> i\<in>{0..<24}.(nprocs_key !! i \<or> n  !! i) \<noteq> nprocs_key !! i"
+  hence "\<exists> i\<in>{0..<proc_id_len}.(@nprocs !! i \<or> n  !! i) \<noteq> @nprocs !! i"
     using nprocs_key_low_zeros proc_id_low_one
     by fast
   thus ?thesis by (force simp add:word_eq_iff word_ao_nth)
 qed
 
-text \<open>Thus @{const nprocs_key} doesn't belong to the set of procedure key addresses.\<close>
-lemma nprocs_key_notin_proc_key_addrs: "\<turnstile> \<S> \<Longrightarrow> nprocs_key \<notin> proc_key_addrs \<S>"
+text \<open>Thus @{text "@nprocs"} doesn't belong to the set of procedure key addresses.\<close>
+lemma nprocs_key_notin_proc_key_addrs: "\<turnstile> \<sigma> \<Longrightarrow> @nprocs \<notin> @proc_keys \<sigma>"
   using proc_id_bounded proc_key_addr_neq_nprocs_key
-  unfolding proc_key_addrs_def
+  unfolding proc_key_addrs_def proc_key_addr_def
   by auto
+
+text \<open>Also procedure index address is different from the address of the \# of procedures
+      (@{text "@nprocs"}).\<close>
+lemma proc_id_addr_neq_nprocs_key: "@proc_id k \<noteq> @nprocs"
+proof
+  have 0: "\<not> @nprocs !! 0" by auto
+  have 1: "@proc_id k !! 0" using lsb0 test_bit_1 by blast
+  assume "@proc_id k = @nprocs"
+  hence "(@proc_id k !! 0) = (@nprocs !! 0)" by auto
+  thus "False" using 0 1 by auto
+qed
+
+text \<open>Thus @{text "@nprocs"} doesn't belong to the set of procedure index addresses.\<close>
+lemma nprocs_key_notin_proc_id_addrs: "\<turnstile> \<sigma> \<Longrightarrow> @nprocs \<notin> @proc_ids \<sigma>"
+  unfolding proc_id_addrs_def
+proof
+  assume assms: "\<turnstile> \<sigma>" and "@nprocs \<in> {@proc_id k |k. k \<in> proc_keys \<sigma>}"
+  hence "\<exists>k. @nprocs = @proc_id k \<and> k \<in> proc_keys \<sigma>" by blast
+  then obtain k where " @nprocs = @proc_id k \<and> k \<in> proc_keys \<sigma>" by blast
+  thus "False" using proc_id_addr_neq_nprocs_key assms by auto
+qed
 
 text \<open>The function mapping procedure id to the corresponding procedure key
       (in some abstract state):\<close>
-definition "proc_key_of_id \<S> \<equiv> the_inv_into (proc_keys \<S>) (proc_id \<S>)"
+definition "proc_key_of_id \<sigma> \<equiv> the_inv_into (proc_keys \<sigma>) (proc_id \<sigma>)"
 
 text \<open>Invertibility of computing procedure id (by its key) in any abstract state:\<close>
-lemma proc_key_of_id_inv[simp]: "\<lbrakk>\<turnstile>\<S>; k \<in> proc_keys \<S>\<rbrakk> \<Longrightarrow> proc_key_of_id \<S> (proc_id \<S> k) = k"
+lemma proc_key_of_id_inv[simp]: "\<lbrakk>\<turnstile>\<sigma>; k \<in> proc_keys \<sigma>\<rbrakk> \<Longrightarrow> proc_key_of_id \<sigma> (proc_id \<sigma> k) = k"
   unfolding procs_map_wf proc_key_of_id_def
   using the_inv_into_f_f by fastforce
 
 text \<open>For any valid procedure id in any well-formed abstract state there is a procedure key that
      corresponds to the id (this is not so trivial as we keep the reverse mapping in
      the abstract state, the proof is implicitly based on the pigeonhole principle).\<close>
-lemma proc_key_exists: "\<lbrakk>\<turnstile>\<S>; i\<in>{1..nprocs \<S>}\<rbrakk> \<Longrightarrow> \<exists>k\<in>proc_keys \<S>. proc_id \<S> k = i"
+lemma proc_key_exists: "\<lbrakk>\<turnstile>\<sigma>; i\<in>{1..nprocs \<sigma>}\<rbrakk> \<Longrightarrow> \<exists>k\<in>proc_keys \<sigma>. proc_id \<sigma> k = i"
 proof (rule ccontr, subst (asm) bex_simps(8))
-  let ?rng = "{1 .. nprocs \<S>}"
-  let ?prj = "proc_id \<S> ` proc_keys \<S>"
-  assume "\<forall>k\<in>proc_keys \<S>. proc_id \<S> k \<noteq> i"
+  let ?rng = "{1 .. nprocs \<sigma>}"
+  let ?prj = "proc_id \<sigma> ` proc_keys \<sigma>"
+  assume "\<forall>k\<in>proc_keys \<sigma>. proc_id \<sigma> k \<noteq> i"
   hence 0:"i \<notin> ?prj"
     by auto
-  assume "\<turnstile> \<S>"
+  assume "\<turnstile> \<sigma>"
   hence 1:"?prj \<subseteq> ?rng" and 2:"card ?prj = card ?rng"
     unfolding abs_wf_def procs_rng_wf_def procs_map_wf_def
     by (auto simp add: image_subset_iff card_image)
@@ -406,8 +486,14 @@ proof (rule ccontr, subst (asm) bex_simps(8))
 qed
 
 text \<open>The function @{const proc_key_of_id} gives valid procedure ids.\<close>
-lemma proc_key_of_id_in_keys: "\<lbrakk>\<turnstile>\<S>; i\<in>{1..nprocs \<S>}\<rbrakk> \<Longrightarrow> proc_key_of_id \<S> i \<in> proc_keys \<S>"
-  using proc_key_exists the_inv_into_into[of "proc_id \<S>" "proc_keys \<S>" i]
+lemma proc_key_of_id_in_keys[simp]: "\<lbrakk>\<turnstile>\<sigma>; i\<in>{1..nprocs \<sigma>}\<rbrakk> \<Longrightarrow> proc_key_of_id \<sigma> i \<in> proc_keys \<sigma>"
+  using proc_key_exists the_inv_into_into[of "proc_id \<sigma>" "proc_keys \<sigma>" i]
+  unfolding proc_key_of_id_def procs_map_wf
+  by fast
+
+text \<open>Invertibility of computing procedure key (by its id) in any abstract state:\<close>
+lemma proc_key_of_id_inv'[simp]: "\<lbrakk>\<turnstile>\<sigma>; i\<in>{1..nprocs \<sigma>}\<rbrakk> \<Longrightarrow> proc_id \<sigma> (proc_key_of_id \<sigma> i) = i"
+  using proc_key_exists f_the_inv_into_f[of "proc_id \<sigma>" "proc_keys \<sigma>" i]
   unfolding proc_key_of_id_def procs_map_wf
   by fast
 
@@ -415,77 +501,167 @@ subsection \<open>Any well-formed abstract state can be stored\<close>
 
 text \<open>A mapping of addresses with specified (defined) values:\<close>
 definition
-  "con_wit_map \<S> :: _ \<rightharpoonup> word32 \<equiv>
-        [nprocs_key \<mapsto> of_nat (nprocs \<S>)]
-     ++ (Some \<circ> ucast \<circ> proc_key_of_id \<S> \<circ> id_of_key_addr) |` proc_key_addrs \<S>"
+  "con_wit_map \<sigma> :: _ \<rightharpoonup> word32 \<equiv>
+        [@nprocs \<mapsto> of_nat (nprocs \<sigma>)]
+     ++ (Some \<circ> ucast \<circ> proc_key_of_id \<sigma> \<circ> id_of_proc_key_addr) |` @proc_keys \<sigma>
+     ++ (Some \<circ> ucast \<circ> proc_key_of_id_addr) |` @proc_ids \<sigma>"
 
 text \<open>A sample storage extending the above mapping with default zero values:\<close>
-definition "con_wit \<S> \<equiv> override_on zero_con (the \<circ> con_wit_map \<S>) (dom (con_wit_map \<S>))"
+definition "con_wit \<sigma> \<equiv> override_on zero_storage (the \<circ> con_wit_map \<sigma>) (dom (con_wit_map \<sigma>))"
 
 lemmas con_wit = con_wit_def con_wit_map_def comp_def
 
-lemma restrict_subst[simp]: "k \<in> S \<Longrightarrow> (f |` { g k | k. k \<in> S}) (g k) = f (g k)"
+lemma restrict_subst[simp]: "k \<in> s \<Longrightarrow> (f |` { g k | k. k \<in> s}) (g k) = f (g k)"
   unfolding restrict_map_def
   by auto
 
+lemma restrict_rule: "x \<notin> A \<Longrightarrow> x \<notin> dom(f |` A)"
+  by simp
+
 text \<open>Existence of a storage corresponding to any well-formed abstract state:\<close>
-theorem models_nonvac: "\<turnstile> \<S> \<Longrightarrow> \<exists> S. S \<tturnstile> \<S>"
-  unfolding models_nprocs models_proc_keys
-proof (intro exI[of _ "con_wit \<S>"] conjI)
-  assume wf:"\<turnstile>\<S>"
-  thus "unat (con_wit \<S> nprocs_key) = nprocs \<S>"
+theorem models_nonvac: "\<turnstile> \<sigma> \<Longrightarrow> \<exists>s. s \<tturnstile> \<sigma>"
+  unfolding models_nprocs models_proc_keys models_proc_ids
+proof (intro exI[of _ "con_wit \<sigma>"] conjI)
+  assume wf:"\<turnstile>\<sigma>"
+  thus "unat (con_wit \<sigma> @nprocs) = nprocs \<sigma>"
     unfolding con_wit
-    using nprocs_key_notin_proc_key_addrs le_unat_uoi[where z=max_nprocs_word]
-    by (subst override_on_apply_in, simp)
-      (subst map_add_dom_app_simps(3), auto simp add:procs_rng_wf)
-  from wf have "\<And> k. k \<in> proc_keys \<S> \<Longrightarrow>
-                     proc_key_of_id \<S> (id_of_key_addr (key_addr_of_id (proc_id \<S> k))) = k"
-    by (subst id_of_key_addr_inv)
-      (auto simp add:procs_rng_wf, force)
-  thus "\<forall>k\<in>proc_keys \<S>. con_wit \<S> (key_addr_of_id (proc_id \<S> k)) = ucast k"
-    unfolding con_wit proc_key_addrs_def
-    by (intro ballI, subst override_on_apply_in, (auto)[1])
-       (subst map_add_find_right, subst restrict_subst, auto)
+    using nprocs_key_notin_proc_key_addrs nprocs_key_notin_proc_id_addrs le_unat_uoi[where z=max_nprocs_word]
+    apply (subst override_on_apply_in, simp, subst map_add_dom_app_simps(3))
+    apply (rule restrict_rule, auto, subst map_add_dom_app_simps(3))
+    by (auto simp add:procs_rng_wf)
+  from wf have "\<And> k. k \<in> proc_keys \<sigma> \<Longrightarrow>
+                     proc_key_of_id \<sigma> (id_of_proc_key_addr (@proc_key (proc_id \<sigma> k))) = k"
+    by (subst id_of_key_addr_inv) (auto simp add:procs_rng_wf, force)
+  thus "\<forall>k\<in>proc_keys \<sigma>. con_wit \<sigma> (@proc_key (proc_id \<sigma> k)) = ucast k"
+    unfolding con_wit proc_key_addrs_def proc_id_addrs_def
+    apply (intro ballI, subst override_on_apply_in, (auto)[1])
+    apply (subst map_add_dom_app_simps(3))
+    (*apply (subst map_add_find_right)
+    apply (subst restrict_subst)
+    by auto *)
+    sorry
+  show "\<forall>k\<in>proc_keys \<sigma>. unat (con_wit \<sigma> (@proc_id k)) = proc_id \<sigma> k"
+    unfolding con_wit proc_key_addrs_def proc_id_addrs_def
+    sorry
 qed
 
-(*TODO: 
-        Prove the encoding is unambiguous i.e.
-        the same storage cannot model two distinct abstract states.
-*)
+subsection \<open>Unambiguity of encoding\<close>
+
+subsubsection \<open>Auxiliary lemmas\<close>
+
+proposition word32_key_downcast:"is_down (ucast :: word32 \<Rightarrow> key)"
+  unfolding is_down_def target_size_def source_size_def
+  by simp
+
+lemmas key_upcast =
+  ucast_down_ucast_id[OF word32_key_downcast]
+  down_ucast_inj[OF word32_key_downcast]
+
+lemma con_id_inj[consumes 4]:
+  "\<lbrakk>\<turnstile> \<sigma>; s \<tturnstile> \<sigma>;
+    i\<^sub>1\<in>{1..nprocs \<sigma>}; i\<^sub>2\<in>{1..nprocs \<sigma>};
+    s (@proc_key i\<^sub>1) = s (@proc_key i\<^sub>2)\<rbrakk> \<Longrightarrow> i\<^sub>1 = i\<^sub>2"
+  unfolding models_proc_keys
+  using proc_key_of_id_in_keys key_upcast
+        proc_key_of_id_inv'[symmetric, of _ i\<^sub>1] proc_key_of_id_inv'[symmetric, of _ i\<^sub>2]
+  by metis
+
+text \<open>
+  The concrete encoding of abstract storage is unambiguous, i. e. the same storage cannot
+  model two distinct well-formed abstract states.
+\<close>
+theorem models_inj[simp]: "\<lbrakk>\<turnstile> \<sigma>\<^sub>1; \<turnstile> \<sigma>\<^sub>2; s \<tturnstile> \<sigma>\<^sub>1; s \<tturnstile> \<sigma>\<^sub>2\<rbrakk> \<Longrightarrow> (\<sigma>\<^sub>1 :: ('p :: proc_class) abs) = \<sigma>\<^sub>2"
+  (is "\<lbrakk>?wf1; ?wf2; ?models1; ?models2\<rbrakk> \<Longrightarrow> _")
+proof (intro abs.equality ext option.expand, rule ccontr)
+  fix x
+  {
+    fix \<sigma> \<sigma>':: "'p abs"
+    assume wf1:"\<turnstile> \<sigma>" and wf2:"\<turnstile> \<sigma>'"
+    assume models1:"s \<tturnstile> \<sigma>" and models2:"s \<tturnstile> \<sigma>'"
+    fix i p
+    assume Some:"procs \<sigma> x = Some (i, p)"
+    with wf1 have "i\<in>{1..nprocs \<sigma>}" unfolding procs_rng_wf Ball_def by auto
+    with wf2 models1 models2
+    have "proc_key_of_id \<sigma>' i \<in> proc_keys \<sigma>' \<and> proc_id \<sigma>' (proc_key_of_id \<sigma>' i) = i"
+      unfolding models_nprocs by simp
+    moreover with Some models1 models2 have "proc_key_of_id \<sigma>' i = x"
+      unfolding models_proc_keys
+      using key_upcast by (metis domI fst_conv option.sel)
+    ultimately have "procs \<sigma>' x \<noteq> None" by auto
+  }
+  note wlog = this
+  assume ?wf1 ?wf2 ?models1 and ?models2
+  {
+    assume neq:"(procs \<sigma>\<^sub>1 x = None) \<noteq> (procs \<sigma>\<^sub>2 x = None)"
+    show False
+    proof (cases "procs \<sigma>\<^sub>1 x")
+      case Some
+      with wlog \<open>?wf1\<close> \<open>?wf2\<close> \<open>?models1\<close> \<open>?models2\<close> neq show ?thesis by fastforce
+    next
+      case None
+      with neq have "procs \<sigma>\<^sub>2 x \<noteq> None" by simp
+      with wlog \<open>?wf1\<close> \<open>?wf2\<close> \<open>?models1\<close> \<open>?models2\<close> neq show ?thesis by force
+    qed
+  }
+  {
+    assume in\<sigma>\<^sub>1:"procs \<sigma>\<^sub>1 x \<noteq> None" and in\<sigma>\<^sub>2:"procs \<sigma>\<^sub>2 x \<noteq> None"
+    show "proc \<sigma>\<^sub>1 x = proc \<sigma>\<^sub>2 x"
+    proof
+      let ?i\<^sub>1 = "proc_id \<sigma>\<^sub>1 x" and ?i\<^sub>2 = "proc_id \<sigma>\<^sub>2 x"
+      from in\<sigma>\<^sub>1 and in\<sigma>\<^sub>2
+      have "procs \<sigma>\<^sub>1 x = Some (?i\<^sub>1, proc_bdy \<sigma>\<^sub>1 x)"
+        and "procs \<sigma>\<^sub>2 x = Some (?i\<^sub>2, proc_bdy \<sigma>\<^sub>2 x)"
+        by auto
+      with \<open>?wf1\<close> and \<open>?wf2\<close>
+      have "?i\<^sub>1\<in>{1..nprocs \<sigma>\<^sub>1}" and "?i\<^sub>2\<in>{1..nprocs \<sigma>\<^sub>2}" unfolding procs_rng_wf by auto
+      moreover with in\<sigma>\<^sub>1 in\<sigma>\<^sub>2 \<open>?models1\<close> and \<open>?models2\<close>
+      have "s (@proc_key ?i\<^sub>1) = s (@proc_key ?i\<^sub>2)" unfolding models_proc_keys by force
+      moreover with \<open>?models1\<close> \<open>?models2\<close> and \<open>?i\<^sub>2\<in>{1..nprocs \<sigma>\<^sub>2}\<close>
+      have "?i\<^sub>2\<in>{1..nprocs \<sigma>\<^sub>1}" unfolding models_nprocs by simp
+      ultimately show "?i\<^sub>1 = ?i\<^sub>2" using \<open>?wf1\<close> \<open>?models1\<close> and con_id_inj[of \<sigma>\<^sub>1] by blast
+
+      show "proc_bdy \<sigma>\<^sub>1 x = proc_bdy \<sigma>\<^sub>2 x"
+        using in\<sigma>\<^sub>1 in\<sigma>\<^sub>2 \<open>?wf1\<close> \<open>?wf2\<close> key_inj
+        unfolding procs_rng_wf by (metis UNIV_I domIff the_inv_into_f_f)
+    qed
+  }
+qed (simp)
 
 section \<open>Well-formedness of a storage state\<close>
 text \<open>
   We need a decoding function on storage states. However, not every storage state can be
-  decoded into an abstract state. So we introduce a minimal well-formedness predicate on 
+  decoded into an abstract state. So we introduce a minimal well-formedness predicate on
   storage states.
 \<close>
 
 text \<open>Number of procedures is bounded, otherwise procedure key addresses can become invalid and we
       cannot read the procedure keys from the storage.\<close>
-definition "nprocs_wf S \<equiv> unat (S nprocs_key) \<le> max_nprocs_nat"
+definition "nprocs_wf s \<equiv> unat (s @nprocs) \<le> max_nprocs"
 
 text \<open>Well-formedness of procedure keys:
       \begin{enumerate}
       \item procedure keys should fit into 24-byte words;
       \item they should represent some existing procedures
-            (currently this essentially a temorary work-around
+            (currently this is essentially a temporary work-around
              and is understood in a very abstract sense
              (Hilbert epsilon operator is used to ``retrieve'' procedures),
              really we need to formalize how the procedures themselves are stored);
-      \item the same procedure key should not be stored by two distinct procedure key addresses.
+      \item the same procedure key should not be stored by two distinct procedure key addresses;
+      \item procedure heap should contain valid procedure index for each procedure key.
       \end{enumerate}\<close>
-definition "proc_keys_wf (dummy :: 'a itself) (S :: storage) \<equiv>
-    (\<forall>k\<in>{S (key_addr_of_id i) | i. i\<in>{1..unat (S nprocs_key)}}. ucast (ucast k :: key) = k)
-  \<and> (\<forall>i\<in>{1..unat (S nprocs_key)}. \<exists>p :: ('a :: proc_class). ucast (key p) = S (key_addr_of_id i))
-  \<and> inj_on (S \<circ> key_addr_of_id) {1..unat (S nprocs_key)}"
+definition "proc_keys_wf (dummy :: 'a itself) (s :: storage) \<equiv>
+    (\<forall>k\<in>{s (@proc_key i) | i. i\<in>{1..unat (s @nprocs)}}. ucast (ucast k :: key) = k)
+  \<and> (\<forall>i\<in>{1..unat (s @nprocs)}. \<exists>p :: ('a :: proc_class). ucast (key p) = s (@proc_key i))
+  \<and> inj_on (s \<circ> @proc_key) {1..unat (s @nprocs)}
+  \<and> (\<forall>i \<in> {1 .. unat (s @nprocs)}. unat (s (@proc_id (ucast (s (@proc_key i))))) = i)"
 
 text \<open>Well-formedness of a storage state: the two above requirements should hold.\<close>
-definition con_wf ("\<TTurnstile>\<^bsub>_\<^esub>_" [60])  where
-  "\<TTurnstile>\<^bsub>(d :: ('a :: proc_class) itself)\<^esub> S \<equiv>
-    nprocs_wf S
-  \<and> proc_keys_wf d S"
+definition con_wf ("\<TTurnstile>\<^bsub>_\<^esub> _" [1000, 60] 60)  where
+  "\<TTurnstile>\<^bsub>(d :: ('a :: proc_class) itself)\<^esub> s \<equiv>
+    nprocs_wf s
+  \<and> proc_keys_wf d s"
 
-notation (input) con_wf ("\<TTurnstile>\<^sub>__" [60])
+notation (input) con_wf ("\<TTurnstile>\<^sub>__" [1000, 60] 60)
 
 lemmas nprocs_wf = con_wf_def nprocs_wf_def
 
@@ -498,127 +674,221 @@ subsection \<open>Auxiliary lemmas\<close>
 
 text \<open>Any property on procedure ids can be reformulated on the corresponding procedure keys
       according to a well-formed abstract state (elimination rule for procedure ids).\<close>
-lemma elim_proc_id:
-  assumes "i \<in> {1..unat (S nprocs_key)}"
-  assumes "\<turnstile> \<S>"
-  assumes "S \<tturnstile> \<S>"
-  obtains k where "k \<in> proc_keys \<S> \<and> i = proc_id \<S> k"
+lemma elim_proc_id[consumes 3]:
+  assumes "i \<in> {1..unat (s @nprocs)}"
+  assumes "\<turnstile> \<sigma>"
+  assumes "s \<tturnstile> \<sigma>"
+  obtains k where "k \<in> proc_keys \<sigma> \<and> i = proc_id \<sigma> k"
   using assms proc_key_exists
   unfolding models_nprocs
   by metis
 
-lemmas key_upcast =
-  ucast_down_ucast_id
-  [where ?'b=256 and ?'a=192,
-   simplified is_down_def target_size_def source_size_def]
-  down_ucast_inj
-  [where ?'b=256 and ?'a=192,
-   simplified is_down_def target_size_def source_size_def]
-
 subsection \<open>Storage corresponding to a well-formed state is well-formed\<close>
-theorem model_wf:"\<lbrakk>\<turnstile>(\<S> :: ('p :: proc_class) abs); S \<tturnstile> \<S>\<rbrakk> \<Longrightarrow> \<TTurnstile>\<^bsub>TYPE ('p)\<^esub>S"
+theorem model_wf[simp, intro]:"\<lbrakk>\<turnstile>(\<sigma> :: ('p :: proc_class) abs); s \<tturnstile> \<sigma>\<rbrakk> \<Longrightarrow> \<TTurnstile>\<^bsub>(p :: 'p itself)\<^esub>s"
   unfolding proc_keys_wf
 proof (intro conjI ballI)
-  assume wf:"\<turnstile> \<S>" and models:"S \<tturnstile> \<S>"
-  thus "nprocs_wf S"
+  assume wf:"\<turnstile> \<sigma>" and models:"s \<tturnstile> \<sigma>"
+  thus "nprocs_wf s"
     unfolding procs_rng_wf models_nprocs nprocs_wf_def by simp
-  show "inj_on (S \<circ> key_addr_of_id) {1..unat (S nprocs_key)}"
+  note elim_id = elim_proc_id[OF _ wf models]
+  show "inj_on (s \<circ> @proc_key) {1..unat (s @nprocs)}"
     unfolding inj_on_def
   proof (intro ballI impI)
     fix x y
-    assume "x\<in>{1..unat (S nprocs_key)}" and "y\<in>{1..unat (S nprocs_key)}"
+    assume "x\<in>{1..unat (s @nprocs)}" and "y\<in>{1..unat (s @nprocs)}"
     from wf models and this
-    show "(S \<circ> key_addr_of_id) x = (S \<circ> key_addr_of_id) y \<Longrightarrow> x = y"
+    show "(s \<circ> @proc_key) x = (s \<circ> @proc_key) y \<Longrightarrow> x = y"
       using key_upcast
-      by (elim elim_proc_id[where \<S>=\<S>]) (auto simp add:models_proc_keys)
+      by (elim elim_id, auto simp add:models_proc_keys)
   qed
-  fix i
-  assume "i\<in>{1..unat (S nprocs_key)}"
-  thus "\<exists>p :: 'p. ucast (key p) = S (key_addr_of_id i)"
-    using wf models
-    by (intro exI[of _ "proc_bdy \<S> (proc_key_of_id \<S> i)"], elim elim_proc_id)
-      (simp+, simp add:models_proc_keys procs_rng_wf)
-next
-  fix k
-  assume wf:"\<turnstile> \<S>" and models:"S \<tturnstile> \<S>"
-  assume "k\<in>{S (key_addr_of_id i) | i. i\<in>{1..unat (S nprocs_key)}}"
-  thus "ucast (ucast k :: key) = k"
-  proof (simp only:Setcompr_eq_image image_iff, elim bexE)
-    fix x
-    assume "x \<in> {1..unat (S nprocs_key)}" and "k = S (key_addr_of_id x)"
+  {
+    fix i
+    assume "i\<in>{1..unat (s @nprocs)}"
+
+    thus "\<exists>p :: 'p. ucast (key p) = s (@proc_key i)"
+      using wf models
+      apply (intro exI[of _ "proc_bdy \<sigma> (proc_key_of_id \<sigma> i)"])
+      by (elim elim_id, simp add:models_proc_keys procs_rng_wf)
+  }
+  {
+    fix k
+    assume "k\<in>{s (@proc_key i) | i. i\<in>{1..unat (s @nprocs)}}"
+    then obtain x where "x \<in> {1..unat (s @nprocs)}" and "k = s (@proc_key x)"
+      by (simp only:Setcompr_eq_image image_iff, elim bexE)
     thus "ucast (ucast k :: key) = k"
       using wf models key_upcast
-      by (elim elim_proc_id[where \<S>=\<S>])
-        (auto simp add:models_proc_keys)
-  qed
+      by (elim elim_id, auto simp add:models_proc_keys)
+  }
+  fix i
+  assume "i \<in> {1..unat (s @nprocs)}"
+  thus "unat (s (@proc_id (ucast (s (@proc_key i))))) = i"
+    using wf models
+    sorry
 qed
 
 section \<open>Decoding of storage\<close>
 
 text \<open>Auxiliary abbreviations\<close>
 
-abbreviation "proc_pair S i \<equiv> (ucast (S (key_addr_of_id i)) :: key, (i, SOME p. True))"
+abbreviation "proc_pair (p :: ('p :: proc_class) itself) s i \<equiv>
+  let k = ucast (s (@proc_key i)) in (k, (i, SOME p :: 'p. key p = k))"
 
-abbreviation "proc_list S \<equiv> [proc_pair S i. i \<leftarrow> [1..<Suc (unat (S nprocs_key))]]"
+abbreviation "proc_list p s \<equiv> [proc_pair p s i. i \<leftarrow> [1..<Suc (unat (s @nprocs))]]"
 
 text \<open>The decoding function:\<close>
-definition abs ("\<lbrace>_\<rbrace>") where "\<lbrace>S\<rbrace> = \<lparr> procs = map_of (proc_list S) \<rparr>"
+definition abs ("\<lbrace>_\<rbrace>\<^bsub>_\<^esub>" [1000, 1000] 1000) where "\<lbrace>s\<rbrace>\<^bsub>p\<^esub> = \<lparr> procs = map_of (proc_list p s) \<rparr>"
 
-lemma inj_on_fst: "inj_on f A \<Longrightarrow> inj_on (\<lambda> x. (f x, y x)) A"
-  unfolding inj_on_def by simp
+notation (input) abs ("\<lbrace>_\<rbrace>\<^sub>_" [1000, 1000] 1000)
 
-(*
-theorem models_abs: "\<TTurnstile>\<^sub>p S \<Longrightarrow> S \<tturnstile> \<lbrace>S\<rbrace>"
-  unfolding models_nprocs models_proc_keys
+lemmas abs_simps =
+  Let_def set_map image_iff set_upt atLeastLessThanSuc_atLeastAtMost
+  abs.simps option.sel fst_conv
+
+theorem models_abs[simp, intro]: "\<TTurnstile>\<^sub>p s \<Longrightarrow> s \<tturnstile> \<lbrace>s\<rbrace>\<^sub>p"
+  unfolding models_nprocs models_proc_keys models_proc_ids
 proof (intro conjI ballI)
-  assume wf:"\<TTurnstile>\<^sub>p S"
-  hence key_inj:"inj_on (\<lambda>i. ucast (S (key_addr_of_id i)) :: key) {1..unat (S nprocs_key)}"
+  assume wf:"\<TTurnstile>\<^sub>p s"
+  hence "inj_on (\<lambda>i. ucast (s (@proc_key i)) :: key) {1..unat (s @nprocs)}"
     unfolding inj_on_def proc_keys_wf
     by (auto simp only:comp_apply Ball_def mem_Collect_eq) metis
-  hence fst_inj:"inj_on fst (set (proc_list S))"
-    unfolding inj_on_def set_map set_upt Ball_def image_iff
+  hence fst_inj:"inj_on fst (set (proc_list p s))"
+    unfolding inj_on_def set_upt Ball_def abs_simps
     by simp
-  moreover have dist:"distinct (proc_list S)"
-    by (simp add:distinct_map inj_on_def)
-  ultimately show "unat (S nprocs_key) = nprocs \<lbrace>S\<rbrace>"
+  have dist:"distinct (proc_list p s)"
+    by (simp add:distinct_map inj_on_def Let_def)
+  show models_nprocs:"unat (s @nprocs) = nprocs \<lbrace>s\<rbrace>\<^sub>p"
     unfolding abs_def
-    by (simp only:abs.simps dom_map_of_conv_image_fst distinct_card[OF dist] card_image[OF fst_inj]
-                  length_map length_upt)
-  fix k
-  assume "k\<in>proc_keys \<lbrace>S\<rbrace>"
-  hence "map_of (proc_list S) k = Some (proc \<lbrace>S\<rbrace> k)"
-    using key_inj fst_inj
-    apply (intro  map_of_is_SomeI)
-     apply (auto simp only:distinct_map, simp)
-     apply (simp only:inj_on_fst set_upt atLeastLessThanSuc_atLeastAtMost)
+    by (simp only:abs.simps dom_map_of_conv_image_fst
+        distinct_card[OF dist] card_image[OF fst_inj] length_map length_upt)
 
-  show "S (key_addr_of_id (proc_id \<lbrace>S\<rbrace> k)) = ucast k"
+  have proc_pair_inj:"inj_on (proc_pair p s) {1..unat (s @nprocs)}"
+    unfolding inj_on_def prod.inject Let_def by simp
+  fix k
+  {
+    fix i q
+    assume proc:"procs \<lbrace>s\<rbrace>\<^sub>p k = Some (i, q)"
+    hence "(k, proc \<lbrace>s\<rbrace>\<^sub>p k) = proc_pair p s i"
+      by (simp only:abs.simps abs_def) (frule map_of_SomeD, auto simp add:Let_def)
+  } note proc_k_eq = this
+  {
+  assume k_in_keys:"k\<in>proc_keys \<lbrace>s\<rbrace>\<^sub>p"
+  hence proc_id_in_range:"proc_id \<lbrace>s\<rbrace>\<^sub>p k \<in> {1..nprocs \<lbrace>s\<rbrace>\<^sub>p}"
+    apply (subst models_nprocs[symmetric])
+    unfolding abs_def by (auto simp only:abs_simps; frule map_of_SomeD)+
+  have "map_of (proc_list p s) k = Some (proc \<lbrace>s\<rbrace>\<^sub>p k)"
+    using fst_inj proc_pair_inj proc_k_eq k_in_keys
+    apply (auto simp only:distinct_map distinct_upt abs_simps intro!:map_of_is_SomeI)
+    using models_nprocs proc_id_in_range
+    by (intro bexI[of _ "proc_id \<lbrace>s\<rbrace>\<^bsub>p\<^esub> k"], simp+)
+  thus "s (@proc_key (proc_id \<lbrace>s\<rbrace>\<^sub>p k)) = ucast k"
     unfolding abs_def
-    apply (simp only:abs.simps)
-    apply (cases "map_of (proc_list S) k")
-    apply (subst map_of_eq_Some_iff)
+    apply (cases "map_of (proc_list p s) k")
+    apply (auto simp only: abs_simps, frule map_of_SomeD)
+    using wf unfolding proc_keys_wf by (force simp only: abs_simps)
+  }
+  next
+  fix k
+  assume "k \<in> proc_keys \<lbrace>s\<rbrace>\<^sub>p"
+  thus "unat (s (@proc_id k)) = proc_id \<lbrace>s\<rbrace>\<^sub>p k"
+    sorry
 qed
-*)
 
 section \<open>System calls\<close>
 
-text \<open>
-  This section will contain specifications of the system calls, but for now there are only some
-  early experiments.
-\<close>
+text \<open>This section will contain specifications of the system calls.\<close>
+
+locale syscall =
+  fixes arg_wf :: "'p :: proc_class abs \<Rightarrow> 'b \<Rightarrow> bool" ("_ \<turnstile> _" [60, 60] 60)
+  fixes arg_abs :: "'a \<Rightarrow> 'b" ("\<lbrace>_\<rbrace>")
+  fixes pre :: "'a \<Rightarrow> storage \<Rightarrow> bool"
+  fixes post :: "'a \<Rightarrow> storage \<Rightarrow> storage \<Rightarrow> bool"
+  fixes app :: "'b \<Rightarrow> 'p abs \<Rightarrow> 'p abs"
+  assumes preserves_wf: "\<lbrakk>\<turnstile>\<sigma>; \<sigma> \<turnstile> arg\<rbrakk> \<Longrightarrow> \<turnstile> app arg \<sigma>"
+  assumes preserves_wf': "\<lbrakk>\<TTurnstile>\<^sub>p s; \<turnstile>\<lbrace>s\<rbrace>\<^sub>p; pre a s; post a s s'\<rbrakk> \<Longrightarrow> \<TTurnstile>\<^sub>p s'"
+  assumes arg_wf: "\<lbrakk>\<TTurnstile>\<^sub>p s; \<turnstile>\<lbrace>s\<rbrace>\<^sub>p; pre a s\<rbrakk> \<Longrightarrow> \<lbrace>s\<rbrace>\<^sub>p \<turnstile> \<lbrace>a\<rbrace>"
+  assumes consistent: "\<lbrakk>\<TTurnstile>\<^sub>p s; \<turnstile>\<lbrace>s\<rbrace>\<^sub>p; pre a s; post a s s'\<rbrakk> \<Longrightarrow> \<lbrace>s'\<rbrace>\<^sub>p = app \<lbrace>a\<rbrace> \<lbrace>s\<rbrace>\<^sub>p"
+begin
+theorem post_wf: "\<lbrakk>\<TTurnstile>\<^sub>p s; \<turnstile>(\<lbrace>s\<rbrace>\<^sub>p :: 'p abs); pre a s; post a s s'\<rbrakk> \<Longrightarrow> \<turnstile>\<lbrace>s'\<rbrace>\<^sub>p"
+  using arg_wf preserves_wf consistent by metis
+end
+
+definition add_proc_arg_wf :: "'p :: proc_class abs \<Rightarrow> (key \<times> 'p) \<Rightarrow> bool" ("_ \<turnstile>\<^bsub>add'_proc\<^esub> _")
+  where
+  "\<sigma> \<turnstile>\<^bsub>add_proc\<^esub> kp \<equiv>
+     let (k, p) = kp in
+     nprocs \<sigma> < max_nprocs \<and>
+     k \<notin> proc_keys \<sigma> \<and>
+     key p = k"
+
+definition "add_proc kp \<sigma> \<equiv> \<sigma> \<lparr> procs := procs \<sigma> (fst kp \<mapsto> (nprocs \<sigma> + 1, snd kp)) \<rparr>"
+
+definition add_proc_arg_abs :: "(key \<times> 'p :: proc_class) \<Rightarrow> (key \<times> 'p)" ("\<lbrace>_\<rbrace>\<^bsub>add'_proc\<^esub>") where
+  "\<lbrace>a\<rbrace>\<^bsub>add_proc\<^esub> = a"
+
+definition
+  "add_proc_pre (kp :: _ \<times> 'p :: proc_class) s \<equiv> \<lbrace>s\<rbrace>\<^bsub>TYPE('p)\<^esub> \<turnstile>\<^bsub>add_proc\<^esub> \<lbrace>kp\<rbrace>\<^bsub>add_proc\<^esub>"
+
+definition
+  "add_proc_post kp s s' \<equiv>
+     let (k, p) = kp in
+     s' @nprocs = s @nprocs + 1 \<and>
+     (\<forall>a\<in>{ @proc_key i | i. i\<in>{1..unat (s @nprocs)}}. s' a = s a) \<and>
+     s' (@proc_key (unat (s @nprocs) + 1)) = k"
+
+lemma add_proc_preserves_wf: "\<lbrakk>\<turnstile>\<sigma>; \<sigma> \<turnstile>\<^bsub>add_proc\<^esub> (k, p)\<rbrakk> \<Longrightarrow> \<turnstile> add_proc (k, p) \<sigma>"
+  (is "\<lbrakk>?wf\<sigma>; ?wf_arg\<rbrakk> \<Longrightarrow> _")
+proof (subst abs_wf_def, unfold procs_rng_wf_def procs_map_wf_def, intro conjI ballI)
+  let ?\<sigma>' = "add_proc (k, p) \<sigma>"
+  assume ?wf\<sigma> and ?wf_arg
+
+  thus "nprocs (?\<sigma>') \<le> max_nprocs" unfolding add_proc_arg_wf_def add_proc_def by simp
+
+  have proc_keys':"proc_keys ?\<sigma>' = proc_keys \<sigma> \<union> {k}"  unfolding add_proc_def by simp
+  have proc_id_k:"proc_id ?\<sigma>' k = nprocs \<sigma> + 1" unfolding add_proc_def by simp
+  have proc_id_unch:"\<forall>k\<in>proc_keys \<sigma>. proc_id ?\<sigma>' k = proc_id \<sigma> k"
+    using \<open>?wf_arg\<close> unfolding add_proc_def add_proc_arg_wf_def by simp
+
+  show "inj_on (proc_id ?\<sigma>') (proc_keys ?\<sigma>')"
+  proof (unfold inj_on_def, intro ballI impI)
+    fix x y
+    assume "x \<in> proc_keys ?\<sigma>'" and "y \<in> proc_keys ?\<sigma>'" and "proc_id ?\<sigma>' x = proc_id ?\<sigma>' y"
+    with \<open>?wf\<sigma>\<close> proc_keys' proc_id_k proc_id_unch show "x = y"
+      unfolding procs_map_wf procs_rng_wf inj_on_def add_proc_arg_wf_def
+                Ball_def atLeastAtMost_iff
+      by (cases "x \<in> proc_keys \<sigma>"; cases "y \<in> proc_keys \<sigma>", auto)
+  qed
+
+  fix k'
+  assume k'_in_keys:"k'\<in>proc_keys ?\<sigma>'"
+
+  with \<open>?wf\<sigma>\<close> \<open>?wf_arg\<close> proc_keys' proc_id_k proc_id_unch
+  show "proc_id ?\<sigma>' k' \<in> {1..nprocs ?\<sigma>'}"
+    unfolding add_proc_arg_wf_def procs_rng_wf Ball_def atLeastAtMost_iff
+    by (cases "k' = k", auto)
+
+  have "proc_bdy ?\<sigma>' k = p" unfolding add_proc_def by simp
+  moreover have "\<forall>k\<in>proc_keys \<sigma>. proc_bdy ?\<sigma>' k = proc_bdy \<sigma> k"
+    using \<open>?wf_arg\<close> unfolding add_proc_def add_proc_arg_wf_def by simp
+  ultimately show "key (proc_bdy ?\<sigma>' k') = k'"
+    using k'_in_keys \<open>?wf\<sigma>\<close> \<open>?wf_arg\<close> proc_keys'
+    unfolding add_proc_arg_wf_def procs_rng_wf
+    by (cases "k' = k", auto)
+qed
+
+subsection \<open>Register Procedure\<close>
+
+text \<open>Early version of "register procedure" operation.\<close>
 
 abbreviation higher32 where "higher32 k n \<equiv> n >> ((32 - k) * 8)"
 
 definition is_kernel_storage_key :: "word32 \<Rightarrow> bool"
   where "is_kernel_storage_key w \<equiv> higher32 4 w = 0xffffffff"
 
-subsection \<open>Register Procedure\<close>
-
 (*
 24 bytes aligned right in the 32 bytes
 *)
 definition n_of_procedures :: "storage \<Rightarrow> word32"
-  where "n_of_procedures s = s nprocs_key"
+  where "n_of_procedures s = s @nprocs"
 
 (*
 When a procedure is added to the kernel:
@@ -628,20 +898,20 @@ When a procedure is added to the kernel:
   4. The length value (the first value) is incremented by one.
   5. TODO: The procedure index value (in procedure metadata) is set to the new length value.
 *)
-definition add_proc :: "key \<Rightarrow> storage \<Rightarrow> storage option"
+definition add_proc' :: "key \<Rightarrow> storage \<Rightarrow> storage option"
   where
-    "add_proc p s \<equiv>
+    "add_proc' p s \<equiv>
       if n_of_procedures s < max_nprocs_word
       then
         Some (s
-              (nprocs_key := n_of_procedures s + 1,
-               nprocs_key OR (n_of_procedures s + 1) := ucast p))
+              (@nprocs := n_of_procedures s + 1,
+               @nprocs OR (n_of_procedures s + 1) := ucast p))
       else
         None"
 
 lemma
   assumes "n_of_procedures s < max_nprocs_word"
-  shows   "case (add_proc p s) of
+  shows   "case (add_proc' p s) of
            Some s' \<Rightarrow> n_of_procedures s' = n_of_procedures s + 1"
 proof-
   have "0 < n_of_procedures s + 1"
@@ -652,27 +922,11 @@ proof-
   moreover have "n_of_procedures s + 1 \<le> max_nprocs_word"
     using assms
     by (metis add.commute add.right_neutral inc_i word_le_sub1 word_not_simps(1) word_zero_le)
-  ultimately have "nprocs_key OR n_of_procedures s + 1 \<noteq> nprocs_key"
+  ultimately have "@nprocs OR n_of_procedures s + 1 \<noteq> @nprocs"
     using proc_key_addr_neq_nprocs_key by auto
   thus ?thesis
-    unfolding add_proc_def
+    unfolding add_proc'_def
     using assms
     by (simp add:n_of_procedures_def)
 qed
-
-section \<open>Tests\<close>
-
-text \<open>
-  These are tests that we use to quickly check that the implemented functions and lemmas are
-  correct, before conducting full-scale proofs.
-\<close>
-
-lemma "(0xFF :: word32) = (255 :: word32)" by auto
-value "is_kernel_storage_key 0xffffffff00000000000000000000000000000000000000000000000000000000"
-value "(0b1011 :: word32) >> 2 = 0x02"
-value "0b1111 :: (2 word)"
-value "ucast (0b1010 :: 4 word) = (0b101010 :: 6 word)"
-value "case (add_proc 5 (\<lambda>x.0)) of (Some s) \<Rightarrow> s nprocs_key"
-value "case (add_proc 5 (\<lambda>x.0)) of (Some s) \<Rightarrow> s (nprocs_key OR 1)"
-value "case (add_proc 5 (\<lambda>x.0)) of (Some s) \<Rightarrow> s (nprocs_key OR 2)"
 end
